WIP: more invariants

dataplane/Examples/Batch_op_Correctness.thy
@@ -10,6 +10,7 @@ imports
   Source_op
   Set_op
 begin
+no_notation shiftr  (infixl \<open>>>\<close> 55)
 
 section \<open>Example\<close>
 
@@ -58,9 +59,9 @@ abbreviation init_operator_state_ty2 where
 
 abbreviation "l1 ip_state \<equiv> ((Logic (ooo_input_op {|1 :: 1|} ip_state) default_internal_summary) :: ('a, _, (_, 't) shared_state + (1 \<Rightarrow> 't antichain), 'c \<times> 't, 't :: {ccompare,canonically_ordered_monoid_add,ordered_ab_semigroup_monoid_add_imp_le,bot}) dataflow_tree)"
 abbreviation "l2 os2 f \<equiv> Logic (batch_op os2 f) default_internal_summary"
-abbreviation "G f ip_state os2 cbuf \<equiv> Comp [(0 :: 2, 1) \<mapsto> (0, 1)] cbuf (l1 (ip_state :: (1, 'd1 + 'd2, 'd1, _) input_state)) (l2 (os2 :: (1, 'd1 + 'd2, 'd1, 'd2, _) operator_state_ty2) f)"
+abbreviation "G f ip_state os2 \<equiv> Comp [(0 :: 2, 1) \<mapsto> (0, 1)] (l1 (ip_state :: (1, 'd1 + 'd2, 'd1, _) input_state)) (l2 (os2 :: (1, 'd1 + 'd2, 'd1, 'd2, _) operator_state_ty2) f)"
 
-abbreviation "test_op \<equiv> compile_dataflow (G (\<lambda> b. if b = [] then trace (STR ''Empty batch! ! !'') [] else [Max (set b)]) (init_input_state default_internal_summary (\<lambda> _. inps_test)) (init_operator_state_ty2 default_internal_summary) (\<lambda> _. []) ) :: (2 \<times> 1, 2 \<times> 1, _) op"
+abbreviation "test_op \<equiv> compile_dataflow (\<lambda> _. []) (G (\<lambda> b. if b = [] then trace (STR ''Empty batch! ! !'') [] else [Max (set b)]) (init_input_state default_internal_summary (\<lambda> _. inps_test)) (init_operator_state_ty2 default_internal_summary) )"
 
 value [GHC] "lmap (\<lambda> io. case io of VOut p (x, t) \<Rightarrow> (projr x, t)) (trace_exec test_op)"
 value [GHC] "check_prefix 100 [((1, 1), (Inr 10, MyPair 1 1)), ((1, 1), (Inr 7, MyPair 0 1)),((1, 1), (Inr 3, MyPair 1 0))] test_op"
@@ -76,8 +77,8 @@ abbreviation "ts inps \<equiv> cimage (\<lambda> e. case e of Data t d \<Rightar
 abbreviation "inp_op os \<equiv> map_op (case_option (Inl (0 :: 2)) (\<lambda> p. Inr (0, p))) (case_option (Inl (0 :: 2)) (\<lambda> p. Inr (0, p))) (ooo_input_op {|1|} os)"
 abbreviation "tt_op os f \<equiv> map_op (case_option (Inl (1 :: 2)) (\<lambda> p. Inr (1, p))) (case_option (Inl (1 :: 2)) (\<lambda> p. Inr (1, p))) (batch_op os f)"
 
-abbreviation "G_op f ip_state os2 cbuf \<equiv>
-   dataflow_tree_to_operator (G f (ip_state :: (1, 'd1 + 'd2, 'd1, _) input_state) (os2 :: (1, 'd1 + 'd2, 'd1, 'd2, _) operator_state_ty2) cbuf)"
+abbreviation "G_op f ip_state os2 chns \<equiv>
+   dataflow_tree_to_operator chns (G f (ip_state :: (1, 'd1 + 'd2, 'd1, _) input_state) (os2 :: (1, 'd1 + 'd2, 'd1, 'd2, _) operator_state_ty2))"
 
 definition "c_pts_inv c caps = (\<forall> l. c_pts c l = caps l)"
 definition "Src_caps_inv caps oss = (\<forall> nid p. caps (Loc nid (Src p)) = zmset_of (mset (ocaps (oss nid) p)))"
@@ -85,7 +86,7 @@ definition "Trg_caps_inv caps bufs = (\<forall> nid p. caps (Loc nid (Trg p)) = 
 definition "extract_prog eds oss = concat (map (\<lambda> nid. extract_progress nid eds (snd (obtain_progress (oss nid)))) Enum.enum)"
 definition "front_inv oss c = (\<forall> nid p. front (oss nid) p \<le> frontier (c_imp c (Loc nid (Trg p))))"
 definition "imp_front_inv su c = (\<forall> l. frontier (c_imp c l) \<le> ifrontier su (+) c l)"
-definition "buf_imp_front_inv su c T nid p = (\<forall> t \<in> T. frontier_less_equal (ifrontier su (+) c (Loc nid (Trg p))) t)"
+definition "chnls_imp_front_inv su c chns = (\<forall> nid p. \<forall> t \<in> snd ` set (chns (nid, p)). frontier_less_equal (ifrontier su (+) c (Loc nid (Trg p))) t)"
 
 definition "propagation_inv su c = 
   (dataflow_topology.inv_imps_work_sum su (-+-) c \<and>
@@ -99,13 +100,14 @@ definition "changes_above_impl_inv su c cgs =
                          (\<forall> (l, t, d) \<in> set cgs'. frontier_less_equal (ifrontier su (+) (change_multiplicities su cgs_l c) l) t)))"
 
 abbreviation "su_test a b \<equiv> dataflow_tree_to_graph (
-    Comp [(0, 0) \<mapsto> (1, 1), (1, 0) \<mapsto> (0, 0)] (\<lambda> _. []) 
-    (Comp [(0, 0) \<mapsto> (0, 0)] (\<lambda> _. []) (Logic (\<oslash> :: (_, _, unit + unit) op) (\<lambda> _ _. [0 :: nat])) (Logic \<oslash> (\<lambda> _ _. [0 :: nat])))
-    (Comp [(0 :: 4, 0 :: 2) \<mapsto> (0, 0)] (\<lambda> _. []) (Logic \<oslash> (\<lambda> _ _. [0 :: nat])) (Logic \<oslash> (\<lambda> _ _. [0 :: nat])))
+    Comp [(0, 0) \<mapsto> (1, 1), (1, 0) \<mapsto> (0, 0)] 
+    (Comp [(0, 0) \<mapsto> (0, 0)] (Logic (\<oslash> :: (_, _, unit + unit) op) (\<lambda> _ _. [0 :: nat])) (Logic \<oslash> (\<lambda> _ _. [0 :: nat])))
+    (Comp [(0 :: 4, 0 :: 2) \<mapsto> (0, 0)] (Logic \<oslash> (\<lambda> _ _. [0 :: nat])) (Logic \<oslash> (\<lambda> _ _. [0 :: nat])))
     ) a b"
 
-definition buff_from_graph where
-  "buff_from_graph su nid p = Set.the_elem { (nid', p'). su (Loc nid' (Src p')) (Loc nid (Trg p)) \<noteq> {}\<^sub>A}"
+
+definition Src_from_Trg where
+  "Src_from_Trg su nid p = Set.the_elem { (nid', p'). su (Loc nid' (Src p')) (Loc nid (Trg p)) \<noteq> {}\<^sub>A}"
 
 lemma correctness_gen:
   fixes inps :: \<open>1 \<Rightarrow> ('t :: {ccompare,canonically_ordered_monoid_add,ordered_ab_semigroup_monoid_add_imp_le,bot}, 'd1) event llist\<close>
@@ -113,43 +115,52 @@ lemma correctness_gen:
     and oss :: \<open>2 \<Rightarrow> (1, 'd1 + 'd2, 't) operator_state\<close>
     and ip_state :: \<open>(1, 'd1 + 'd2, 'd1, 't) input_state\<close>
     and bt_state :: \<open>(1, 'd1 + 'd2, 'd1, 'd2, 't) operator_state_ty2\<close>
+    and chns :: \<open>2 \<times> 1 \<Rightarrow> (('d1 + 'd2) \<times> 't) list\<close>
+    and sg :: \<open>(2, 1, 't) subgraph\<close>
   assumes
     SUBGRAPH_INV:
     \<open>c = pt_tr sg\<close>
-    \<open>summ sg = dataflow_tree_to_graph (G f ip_state bt_state gbuf)\<close>
-    \<open>edges sg = (\<lambda> l. if l = Loc 0 (Src 1) then [Loc 1 (Trg 1)] else [])\<close>
+    \<open>summ sg = dataflow_tree_to_graph (G f ip_state bt_state)\<close>
+    \<open>edges sg = graph_to_edges (summ sg)\<close>
     and
     OP_STATE_INV: 
-    \<open>ip_state = operator_state.extend (oss 1) \<lparr>en1 = Inl, de1 = projl, es = inps\<rparr>\<close>
-    \<open>bt_state = operator_state.extend (oss 2) \<lparr>en1 = Inl, de1 = projl, en2 = Inr, de2 = projr\<rparr>\<close>
+    \<open>ip_state = operator_state.extend (oss 0) \<lparr>en1 = Inl, de1 = projl, es = inps\<rparr>\<close>
+    \<open>bt_state = operator_state.extend (oss 1) \<lparr>en1 = Inl, de1 = projl, en2 = Inr, de2 = projr\<rparr>\<close>
     and
     BUFS_INV: 
-    \<open>outpu (oss 1) 1 = map (\<lambda> (d, t). (Inl d, t)) out_os1\<close>
-    \<open>input (oss 2) 1 = map (\<lambda> (d, t). (Inl d, t)) inp_os2\<close>
-    \<open>buf = out_os1 @ cbuf @ inp_os2\<close>
-    \<open>bufs = (\<lambda> nid p. if nid = 1 \<and> p = 0 then buf else [])\<close>
-    \<open>gbuf = (\<lambda> p. case p of Inl x \<Rightarrow> [] | Inr x \<Rightarrow> map (\<lambda> (d, t). Inr (Inl d, t)) cbuf)\<close>
+    \<open>outchns = (\<lambda> (nid, p). let (nid', p') = Src_from_Trg (summ sg) nid p in outpu (oss nid') p')\<close>
+    \<open>inpchns = (\<lambda> (nid, p). outpu (oss nid) p)\<close>
+    \<open>chns = outchns >> cbufs >> inpchns\<close>
     and
     C_PTS_INV:
     \<open>Src_caps_inv caps oss\<close>
     \<open>Trg_caps_inv caps bufs\<close>
     \<open>cgs = extract_prog (edges sg) oss\<close>
-    \<open>c' = change_multiplicities my_summ cgs c\<close>
+    \<open>c' = change_multiplicities (summ sg) cgs c\<close>
     \<open>c_pts_inv c' caps\<close>
-    \<open>buf_imp_front_inv my_summ c (snd ` set buf) 1 0\<close>
     and
     C_IMP_INV:
     \<open>front_inv oss c\<close>
-    \<open>imp_front_inv my_summ c\<close>
+    \<open>imp_front_inv (summ sg) c\<close>
+    \<open>chnls_imp_front_inv (summ sg) c chns\<close>
     and
     CGS_INV:
-    \<open>changes_above_impl_inv my_summ c cgs\<close>
+    \<open>changes_above_impl_inv (summ sg) c cgs\<close>
     \<open>changes_non_zero_inv cgs\<close>
     and
     PROP_INV:
-    \<open>propagation_inv my_summ c\<close>
+    \<open>propagation_inv (summ sg) c\<close>
+    and
+    INP_STREAM_IN:
+    \<open>timely_input_stream (inps 0) C\<close>
+    \<open>zmset_of C = caps (Loc 0 (Src 0))\<close>
   shows 
-    \<open>set_op S D (dataflow_op sg (G_op f ip_state bt_state gbuf)) \<approx> set_spec_op (cUn S S') D\<close>
+    \<open>set_op S D (dataflow_op sg (G_op f ip_state bt_state cbufs)) \<approx> set_spec_op (cUn S S') D\<close>
+  term "edges sg"
+  term "\<lambda> (nid, p). let (nid', p') = Src_from_Trg (summ sg) nid p in outpu (oss nid') p'"
+  term BULK_BENQ
+  find_consts "_ zmultiset" "_ multiset"
+
   oops
 
 
